SSASlideDG.dfy
@@ -1,0 +1,29 @@
+include "Definitions.dfy"
+include "Util.dfy"
+include "PDG.dfy"
+
+
+// SSASlideDG Definitions:
+datatype SSASlideTag = Phi | Regular
+type SSASlide = (SSASlideTag, CFGNode, Variable, set<CFGNode>)
+type SSAEdge = (SSASlide, SSASlide, set<Variable>)
+type SSASlideDG = (Statement, set<SSASlide>, map<SSASlide, set<SSASlide>>) // map from node to it's predecssors
+
+method ComputeSSASlideDG(S: Statement, pdgN: set<PDGNode>, pdgE: set<PDGEdge>) returns (ssaSlideDG: SSASlideDG)
+{
+	var N := ComputeSSASlideDGNodes(S, pdgN);
+	var E := ComputeSSASlideDGEdges(S, N);
+	var m : map<SSASlide, set<SSASlide>>; // TODO
+
+	//ssaSlideDG := (S, N, E, m);
+}
+
+method ComputeSSASlideDGNodes(S: Statement, pdgN: set<PDGNode>) returns (slides: set<SSASlide>)
+{
+
+}
+
+method ComputeSSASlideDGEdges(S: Statement, Slides: set<SSASlide>) returns (edges: set<SSAEdge>)
+{
+
+}
