SlideDG.dfy
@@ -9,6 +9,7 @@ type Edge = (Slide, Slide, set<Variable>)
 type SlideDG = (Statement, set<Slide>, map<Slide, set<Slide>>) // map from node to it's predecssors
 
 method ComputeSlideDG(S: Statement, pdgN: set<PDGNode>, pdgE: set<PDGEdge>) returns (slideDG: SlideDG)
+	requires Core(S)
 {
 	var N := ComputeSlideDGNodes(S, pdgN);
 	var E := ComputeSlideDGEdges(S, N);
@@ -18,6 +19,7 @@ method ComputeSlideDG(S: Statement, pdgN: set<PDGNode>, pdgE: set<PDGEdge>) retu
 }
 
 method ComputeSlideDGNodes(S: Statement, pdgN: set<PDGNode>) returns (slides: set<Slide>)
+	requires Core(S)
 {
 	slides := {};
 	var copyPDGN := pdgN;
@@ -41,6 +43,7 @@ method ComputeSlideDGNodes(S: Statement, pdgN: set<PDGNode>) returns (slides: se
 }
 
 method ComputeSlideDGEdges(S: Statement, Slides: set<Slide>) returns (edges: set<Edge>)
+	requires Core(S)
 {
 	edges := {};
 	var copySlides := Slides;
@@ -71,60 +74,4 @@ method ComputeSlideDependence(Slides: set<Slide>, Sm: Slide) returns (slideDepSl
 method ComputeSlide(S: Statement, v: Variable, l: Label) returns (n: Slide)
 
 
-
-/*
-/*function FlowInsensitiveSlice(S: Statement, V: set<Variable>): Statement
-	// FIXME: generalize
-	requires S == Assignment(["i","sum", "prod"],["i+1","sum+i","prod*i"])
-{
-	if V == {"sum"} then Assignment(["sum"],["sum+i"])
-	else Assignment(["i","prod"],["i+1","prod*i"])
-}*/
-
-function method GetAssignmentsOfV(LHS : seq<Variable>, RHS : seq<Expression>, V: set<Variable>) : Statement
-
-{
-	if LHS == [] then Skip
-	else if LHS[0] in V then 
-	var tempRes := GetAssignmentsOfV(LHS[1..], RHS[1..], V);
-	match tempRes {
-		case Assignment(LHS1,RHS1) => Assignment([LHS[0]]+LHS1, [RHS[0]]+RHS1)
-	}
-	else GetAssignmentsOfV(LHS[1..], RHS[1..], V)
-
-	/*if LHS == [] then Skip
-	else if LHS[0] in V then SeqComp(Assignment([LHS[0]],[RHS[0]]), GetAssignmentsOfV(LHS[1..], RHS[1..], V))
-	else GetAssignmentsOfV(LHS[1..], RHS[1..], V)*/
-}
-
-function method ComputeSlides(S: Statement, V: set<Variable>) : Statement
-
-{
-	if V * def(S) == {} then Skip
-	else
-	match S {
-		case Skip => Skip
-		case Assignment(LHS,RHS) => GetAssignmentsOfV(LHS,RHS,V)
-		case SeqComp(S1,S2) => SeqComp(ComputeSlides(S1,V), ComputeSlides(S2,V))
-		case IF(B0,Sthen,Selse) => IF(B0, ComputeSlides(Sthen,V) , ComputeSlides(Selse,V))
-		case DO(B,S) => DO(B, ComputeSlides(S,V))
-	}
-}
-
-function method ComputeSlidesDepRtc(S: Statement, V: set<Variable>) : set<Variable>
-
-{
-	var slidesSV := ComputeSlides(S, V);
-	var U := glob(slidesSV) * def(S);
-
-	if U <= V then V else ComputeSlidesDepRtc(S, V + U)
-}
-
-
-method ComputeFISlice(S: Statement, V: set<Variable>) returns (SV: Statement)
-	//ensures SV == FlowInsensitiveSlice(S,V)
-{
-	var Vstar := ComputeSlidesDepRtc(S, V);
-
-	SV := ComputeSlides(S, Vstar);
-}*/
+function SlideDGNeighbours(n: Slide) : set<Slide>
