‏‏SSASlicing.dfy
@@ -1,0 +1,462 @@
+include "Definitions.dfy"
+include "Substitutions.dfy"
+include "Util.dfy"
+include "CorrectnessSSA.dfy"
+include "SSA.dfy"
+include "SlideDG.dfy"
+include "Slicing.dfy"
+
+method SSASlice(S: Statement, V: set<Variable>) returns (res: Statement)
+	requires Valid(S)
+	requires Core(S)
+	decreases *
+{
+	var cfg := ComputeCFG(S);
+	var pdgN, pdgE := ComputePDG(S, cfg); // TODO: Change to PDG
+	var slideDG := ComputeSlideDG(S, pdgN, pdgE);
+
+	res := ComputeSSASlice(S, V, slideDG, cfg);
+}
+
+method ComputeSSASlice(S: Statement, V: set<Variable>, ghost slideDG: SlideDG, ghost cfg: CFG) returns (res: Statement)
+	requires Valid(S)
+	requires Core(S)
+	decreases *
+	ensures Valid(res)
+	ensures Core(res)
+	ensures var slidesSV: set<Slide> := slidesOf(res, V); forall Sm :: Sm in slidesSV <==> Sm in finalDefSlides(S, slideDG, cfg, V) || (exists Sn :: Sn in finalDefSlides(S, slideDG, cfg, V) && SlideDGReachable(Sm, Sn, slideDG.1))	 
+{
+	// To SSA
+	var vsSSA := new VariablesSSA(); 
+	var Xset := def(S);
+	var X := setToSeq(Xset);
+	var Y := {};
+	var liveOnEntryXSeq := freshInit(X, {}, vsSSA);
+	var liveOnEntryX := setOf(liveOnEntryXSeq);
+	var liveOnExitXSeq := freshInit(X, glob(S) + liveOnEntryX, vsSSA);
+	var liveOnExitX := setOf(liveOnExitXSeq);
+	var XLs := liveOnEntryX + liveOnExitX;
+	assert forall i :: i in liveOnEntryX ==> vsSSA.existsVariable2(i);
+	assert forall i :: i in liveOnExitX ==> vsSSA.existsVariable2(i);
+	assert forall v :: v in X ==> vsSSA.existsInstance(v);
+	var S' := ToSSA(S, X, liveOnEntryX, liveOnExitX, Y, XLs, vsSSA);
+
+	// V' := foreach v in V find liveOnExit v
+
+	var V';
+
+	// Flow-Insensitive Slice
+	var S'FI := ComputeFISlice(S', V');
+
+	// From SSA
+	var XL1i := liveOnEntryXSeq;
+	var XL2f := liveOnExitXSeq;
+	res := FromSSA(S'FI, X, XL1i, XL2f, Y, XLs, vsSSA);
+}
+
+function slidesOf(S: Statement, V: set<Variable>) : set<Slide>
+	reads *
+	requires Valid(S)
+	requires Core(S)
+{
+	slidesOf'(S, V, [], {})
+}
+
+function slidesOf'(S: Statement, V: set<Variable>, l: Label, nodes: set<CFGNode>) : set<Slide>
+	reads *
+	requires Valid(S)
+	requires Core(S)
+{
+	match S {
+	case Skip => {}
+	case Assignment(LHS,RHS) => set v | v in V * setOf(LHS) :: (CFGNode.Node(l), v, nodes)
+	case SeqComp(S1,S2) =>		slidesOf'(S1, V, l+[1], nodes) + slidesOf'(S2, V, l+[2], nodes)
+	case IF(B0,Sthen,Selse) =>	slidesOf'(Sthen, V, l+[1], nodes + {CFGNode.Node(l)}) + slidesOf'(Selse, V, l+[2], nodes + {CFGNode.Node(l)})
+	case DO(B,Sloop) =>			slidesOf'(Sloop, V, l+[1], nodes + {CFGNode.Node(l)})
+	}
+}
+
+function statementOf(slides: set<Slide>, S: Statement): Statement
+	reads *
+	requires Valid(S)
+	requires Core(S)
+	requires slides <= allSlides(S)
+	ensures Core(statementOf(slides, S))
+	ensures Valid(statementOf(slides, S))
+	ensures Substatement(statementOf(slides, S), S)
+{
+//Slide = (CFGNode, Variable, set<CFGNode>)
+//CFGNode = Node(l:Label) | Entry | Exit
+
+	if slides == {} then Skip
+	else
+	var slide :| slide in slides;
+	match slide.0 {
+	case Node(l) => 	var S' := statementOfSlide(slide, l, S);
+						var rest := statementOf(slides - {slide}, S);
+						mergeStatements(S', rest, S)
+	case Entry =>		Skip // ?
+	case Exit =>		Skip // ?
+	}
+}
+
+function allSlides(S: Statement) : set<Slide>
+	reads *
+	requires Valid(S)
+	requires Core(S)
+{
+	slidesOf(S, def(S))
+}
+
+function statementOfSlide(slide: Slide, l: Label, S: Statement): Statement
+	reads *
+	requires Valid(S)
+	requires Core(S)
+	requires |l| >= 1
+	//requires ValidLabel(l, S)?
+	ensures Core(statementOfSlide(slide, l, S))
+	ensures Valid(statementOfSlide(slide, l, S))
+	ensures Substatement(statementOfSlide(slide, l, S), S)
+{
+	match S {
+	case Skip => Skip
+	case Assignment(LHS,RHS) => S
+	case SeqComp(S1,S2) =>		if l[0] == 1 then SeqComp(statementOfSlide(slide, l[1..], S1), Skip)  else SeqComp(Skip, statementOfSlide(slide, l[1..], S2))
+	case IF(B0,Sthen,Selse) =>	if l[0] == 1 then IF(B0, statementOfSlide(slide, l[1..], Sthen), Skip) else IF(B0, Skip, statementOfSlide(slide, l[1..], Selse))
+	case DO(B,Sloop) =>			DO(B, statementOfSlide(slide, l[1..], Sloop))
+	}
+}
+
+function mergeStatements(S1: Statement, S2: Statement, S: Statement) : Statement
+	reads *
+	requires Valid(S1)
+	requires Valid(S2)
+	requires Valid(S)
+	requires Core(S)
+	requires Core(S1)
+	requires Core(S2)
+	requires Substatement(S1, S) && Substatement(S2, S) 
+	ensures Valid(mergeStatements(S1, S2, S))
+	ensures Core(mergeStatements(S1, S2, S))
+{
+	match S1 {
+	case Skip =>				  S2
+								  
+	case Assignment(LHS1,RHS1) => match S2 {
+								  case Skip =>					S1
+								  case Assignment(LHS2,RHS2) => match S {
+																case Assignment(LHS',RHS') => var LR := mergeAssignments(LHS1, LHS2, RHS1, RHS2, {}); Assignment(LR.0, LR.1)
+																}
+								  }
+	case SeqComp(S11,S12) =>	  match S2 {
+								  case Skip =>					S1
+								  case SeqComp(S21,S22) =>		match S {
+																case SeqComp(S1',S2') => SeqComp(mergeStatements(S11, S21, S1'), mergeStatements(S12, S22, S2'))
+																}
+								  }
+	case IF(B1,Sthen1,Selse1) =>  match S2 {
+								  case Skip =>					S1
+								  case IF(B2,Sthen2,Selse2) =>	match S {
+																case IF(B',Sthen',Selse') => IF(B1, mergeStatements(Sthen1, Sthen2, Sthen'), mergeStatements(Selse1, Selse2, Selse'))
+																}
+								  }
+	case DO(B1,Sloop1) =>		  match S2 {
+								  case Skip =>					S1 
+								  case DO(B2,Sloop2) =>			match S {
+																case DO(B',Sloop') => DO(B1, mergeStatements(Sloop1, Sloop2, Sloop'))
+																}
+								  }
+	}
+}
+
+function mergeAssignments(LHS1: seq<Variable>, LHS2: seq<Variable>, RHS1: seq<Expression>, RHS2: seq<Expression>, vars: set<Variable>) : (seq<Variable>, seq<Expression>)
+	requires |LHS1| == |RHS1| && |LHS2| == |RHS2|
+	ensures Valid(Assignment(mergeAssignments(LHS1, LHS2, RHS1, RHS2, vars).0, mergeAssignments(LHS1, LHS2, RHS1, RHS2, vars).1))
+{
+	// LHS1 = [x,y]
+	// LHS2 = [y,z]
+	// RHS1 = [1,2]
+	// RHS2 = [2,3]
+
+	// LHS1 = [x,y]
+	// LHS2 = [x,z]
+	// RHS1 = [1,2]
+	// RHS2 = [1,3]
+
+	// LHS1 = [x,y]
+	// LHS2 = [z,x]
+	// RHS1 = [1,2]
+	// RHS2 = [3,1]
+
+	// LHS1 = [x,y,z]
+	// LHS2 = [u,v]
+	// RHS1 = [1,2,3]
+	// RHS2 = [4,5]
+
+
+	if LHS1 == [] && LHS2 == [] then ([],[])
+	else
+		if LHS1 == [] && LHS2 != [] then 
+			var res := mergeAssignments(LHS1, LHS2[1..], RHS1, RHS2[1..], vars + {LHS2[0]});
+			var LHS := [LHS2[0]] + res.0;
+			var RHS := [RHS2[0]] + res.1;
+			(LHS, RHS)			
+		else if LHS1 != [] && LHS2 == [] then
+			var res := mergeAssignments(LHS1[1..], LHS2, RHS1[1..], RHS2, vars + {LHS1[0]});
+			var LHS := [LHS1[0]] + res.0;
+			var RHS := [RHS1[0]] + res.1;
+			(LHS, RHS)			
+		else 
+			if LHS1[0] == LHS2[0] then
+				var res := mergeAssignments(LHS1[1..], LHS2[1..], RHS1[1..], RHS2[1..], vars + {LHS1[0]});
+				var LHS := [LHS1[0]] + res.0;
+				var RHS := [RHS1[0]] + res.1;
+				(LHS, RHS)
+			else
+				var res := mergeAssignments(LHS1[1..], LHS2[1..], RHS1[1..], RHS2[1..], vars + {LHS1[0], LHS2[0]});
+				if LHS1[0] !in vars && LHS2[0] !in vars then
+					var LHS := [LHS1[0]] + [LHS2[0]] + res.0;
+					var RHS := [RHS1[0]] + [RHS2[0]] + res.1;
+					(LHS, RHS)
+				else if LHS1[0] !in vars then
+					var LHS := [LHS1[0]] + res.0;
+					var RHS := [RHS1[0]] + res.1;
+					(LHS, RHS)
+				else /* if LHS2[0] !in vars then */
+					var LHS := [LHS2[0]] + res.0;
+					var RHS := [RHS2[0]] + res.1;
+					(LHS, RHS)
+}
+
+predicate Substatement(S': Statement, S: Statement)
+	reads *
+	requires Valid(S')
+	requires Valid(S)
+	requires Core(S')
+	requires Core(S)
+{
+	match S {
+	case Skip =>				S' == Skip		
+	case Assignment(LHS,RHS) =>	match S' {
+								case Skip => true
+								case Assignment(LHS',RHS') => |LHS'| <= |LHS| && |RHS'| <= |RHS| && assignmentsMatch(LHS, LHS', RHS, RHS')
+								case SeqComp(S1',S2') => false
+								case IF(B0',Sthen',Selse') => false
+								case DO(B',Sloop') => false
+								}
+	case SeqComp(S1,S2) =>		match S' {
+								case Skip => true
+								case Assignment(LHS',RHS') => false
+								case SeqComp(S1',S2') => Substatement(S1', S1) && Substatement(S2', S2)
+								case IF(B0',Sthen',Selse') => false
+								case DO(B',Sloop') => false
+								}	
+	case IF(B0,Sthen,Selse) =>	match S' {
+								case Skip => true
+								case Assignment(LHS',RHS') => false
+								case SeqComp(S1',S2') => false								
+								case IF(B0',Sthen',Selse') => B0 == B0' && Substatement(Sthen', Sthen) && Substatement(Selse', Selse)
+								case DO(B',Sloop') => false
+								}
+	case DO(B,Sloop) =>			match S' {
+								case Skip => true
+								case Assignment(LHS',RHS') => false
+								case SeqComp(S1',S2') => false								
+								case IF(B0',Sthen',Selse') => false
+								case DO(B',Sloop') => B == B' && Substatement(Sloop', Sloop)
+								}
+	}
+}
+
+predicate assignmentsMatch(LHS: seq<Variable>, LHS': seq<Variable>, RHS: seq<Expression>, RHS': seq<Expression>)
+	requires |LHS'| <= |LHS| && |RHS'| <= |RHS| && |LHS'| == |RHS'| && |LHS| == |RHS|
+{
+	// S:   x,y,z := 1,2,3;
+	// S':  z,x := 3,1;
+
+	if LHS' == [] then true
+	else
+		if LHS'[0] !in LHS then false
+		else
+			var i := findVariableInSeq(LHS'[0], LHS);
+			if RHS'[0] != RHS[i] then false
+			else
+				assignmentsMatch(LHS, LHS'[1..], RHS, RHS'[1..])		
+}
+
+function findVariableInSeq(v: Variable, vars: seq<Variable>): int
+	requires v in vars
+	ensures 0 <= findVariableInSeq(v, vars) < |vars|
+{
+	if vars[0] == v then 0
+	else findVariableInSeq(v, vars[1..]) + 1
+}
+
+
+///////////////////////////////////////////////////////////////////////////////////////////////////
+
+
+
+/*if y == 0
+	x := 1;
+else
+	x := 2;
+
+
+
+if y == 0
+	x1 := 1;
+	x3 := x1;
+else
+	x2 := 2;
+	x3 := x2;
+
+
+
+if y == 0
+	x := 1;
+else
+	;
+
+
+if y == 0
+	x1 := 1;
+	;
+else
+	;*/
+
+/*
+// Original S:
+
+i=0
+sum=0
+prod=1
+while i<a.len do
+	sum=sum+a[i]
+	prod=prod*a[i]
+	i=i+1
+od
+i=0
+
+// FISlice Of {prod}
+
+i=0
+
+prod=1
+while i<a.len do
+
+	prod=prod*a[i]
+	i=i+1
+od
+i=0
+
+
+// To SSA:
+
+|[ var i0,sum0,prod0,i1,i4,i7,i8,sum2,sum4,sum5,prod3,prod4,prod6,prod7;
+
+i0,sum0,prod0=i,sum,prod
+
+i1=0
+sum2=0
+prod3=1
+i4,sum4,prod4=i1,sum2,prod3
+while i4<a.len do
+	sum5=sum4+a[i4]
+	prod6=prod4*a[i4]
+	i7=i4+1
+	i4,sum4,prod4=i7,sum5,prod6
+od
+i8=0
+
+i,sum,prod=i8,sum4,prod4 ]|
+
+
+// FISlice:
+
+V={prod}
+V'={prod4}
+
+|[ var i0,sum0,prod0,i1,i4,i7,i8,sum2,sum4,sum5,prod3,prod4,prod6,prod7;
+
+i0,sum0,prod0=i,sum,prod
+
+i1=0
+
+prod3=1
+i4,prod4=i1,prod3
+while i4<a.len do
+	
+	prod6=prod4*a[i4]
+	i7=i4+1
+	i4,prod4=i7,prod6
+od
+
+
+i,sum,prod=i8,sum4,prod4 ]|
+
+glob(slides(prod4))={prod4,prod3,prod6,i4,a}
+U1={prod4,prod3,prod6,i4}
+V1={prod4,prod3,prod6,i4}
+glob(slides(prod4,prod3,prod6,i4))={prod4,prod3,prod6,i1,i4,i7,a}
+U2={prod4,prod3,prod6,i1,i4,i7}
+V2={prod4,prod3,prod6,i1,i4,i7} - VStar
+
+
+// From SSA:
+
+i=0
+prod=1
+while i<a.len do
+	prod=prod*a[i]
+	i=i+1
+od
+
+
+*/
+
+
+function method {:verify false}GetAssignmentsOfV(LHS : seq<Variable>, RHS : seq<Expression>, V: set<Variable>) : Statement
+{
+	if LHS == [] then Skip
+	else if LHS[0] in V then 
+	var tempRes := GetAssignmentsOfV(LHS[1..], RHS[1..], V);
+	match tempRes {
+		case Assignment(LHS1,RHS1) => Assignment([LHS[0]]+LHS1, [RHS[0]]+RHS1)
+	}
+	else GetAssignmentsOfV(LHS[1..], RHS[1..], V)
+
+	/*if LHS == [] then Skip
+	else if LHS[0] in V then SeqComp(Assignment([LHS[0]],[RHS[0]]), GetAssignmentsOfV(LHS[1..], RHS[1..], V))
+	else GetAssignmentsOfV(LHS[1..], RHS[1..], V)*/
+}
+
+function method {:verify false}ComputeSlides(S: Statement, V: set<Variable>) : Statement
+{
+	if V * def(S) == {} then Skip
+	else
+	match S {
+		case Skip => Skip
+		case Assignment(LHS,RHS) => GetAssignmentsOfV(LHS,RHS,V)
+		case SeqComp(S1,S2) => SeqComp(ComputeSlides(S1,V), ComputeSlides(S2,V))
+		case IF(B0,Sthen,Selse) => IF(B0, ComputeSlides(Sthen,V) , ComputeSlides(Selse,V))
+		case DO(B,S) => DO(B, ComputeSlides(S,V))
+	}
+}
+
+function method {:verify false}ComputeSlidesDepRtc(S: Statement, V: set<Variable>) : set<Variable>
+{
+	var slidesSV := ComputeSlides(S, V);
+	var U := glob(slidesSV) * def(S);
+
+	if U <= V then V else ComputeSlidesDepRtc(S, V + U)
+}
+
+
+method {:verify false} ComputeFISlice(S: Statement, V: set<Variable>) returns (SV: Statement)
+	//ensures SV == FlowInsensitiveSlice(S,V)
+{
+	var Vstar := ComputeSlidesDepRtc(S, V);
+
+	SV := ComputeSlides(S, Vstar);
+}
